...

stlc.v
@@ -1,9 +1,12 @@
 
 Require Import Coq.Program.Equality.
+Require Import Lia.
+Require Import Coq.Arith.PeanoNat.
+Require Import Coq.Arith.Compare_dec.
 
 Ltac inv H := dependent destruction H.
 
-Notation "^ f" := (option_map f) (at level 5, right associativity).
+Notation "^ f" := (option_map f) (at level 5, right associativity) : function_scope.
 Notation "^ X" := (option X) : type_scope.
 
 Inductive ty :=
@@ -31,6 +34,8 @@ Notation "x" := x (in custom stlc at level 0, x constr at level 0).
 Notation "0" := (tm_var None) (in custom stlc at level 0).
 Notation "1" := (tm_var (Some None)) (in custom stlc at level 0).
 Notation "2" := (tm_var (Some (Some None))) (in custom stlc at level 0).
+Notation "3" := (tm_var (Some (Some (Some None)))) (in custom stlc at level 0).
+Notation "4" := (tm_var (Some (Some (Some (Some None))))) (in custom stlc at level 0).
 (* Notation "'S' .. 'S' x" := (tm_var (inc_S .. (inc_S x) ..)) (in custom stlc at level 0). *)
 Notation "'var' V" := (tm_var V) (in custom stlc at level 1, left associativity).
 Notation "x y" := (tm_app x y) (in custom stlc at level 1, left associativity).
@@ -75,16 +80,58 @@ Inductive val : term -> Prop :=
 | val_abs : forall e t, val (do \t, e)
 .
 
+(* source: https://github.com/pi8027/lambda-calculus/blob/master/coq/LN/Untyped.v *)
+Require Import Coq.funind.Recdef.
+(* Set Implicit Arguments. *)
+Notation nopts n T := (iter _ n option T).
+
+Notation tm' n V := (tm (nopts n V)).
+Notation term' n := (tm' n Void).
+
+Fixpoint tmap {V1 V2 : Type} (f : V1 -> V2) (e : tm V1) : tm V2 :=
+  match e with
+  | tm_var x => tm_var (f x)
+  | tm_app e1 e2 => tm_app (tmap f e1) (tmap f e2)
+  | tm_abs ty e => tm_abs ty (tmap ^f e)
+  end.
+
+Definition lift {V} (e : tm V) : tm ^V := tmap Some e.
+
+Fixpoint tm_subst_var
+  {V : Type} (n : nat) (e : tm V) : nopts (S n) V -> tm' n V :=
+  match n with
+  | 0 => fun (v : ^V) =>
+      match v with
+      | None => e
+      | Some v => tm_var v
+      end
+  | S n => fun v =>
+      match v with
+      | None => tm_var None
+      | Some v => lift (tm_subst_var n e v)
+      end
+  end.
+
+Fixpoint tm_subst_n
+  {V : Type} (n : nat) (e : tm' (S n) V) (e' : tm V) : tm' n V :=
+  match e with
+  | do var v => tm_subst_var n e' v
+  | do e1 e2 => do {tm_subst_n n e1 e'} {tm_subst_n n e2 e'}
+  | do \t, e => do \t, {tm_subst_n (S n) e e'}
+  end.
+
 (* Substitution *)
 
-Fixpoint lift {V} (e : tm V) : tm ^V :=
+(* Fixpoint lift {V} (e : tm V) : tm ^V :=
   match e with
   | tm_var v => tm_var (Some v)
   | tm_app e1 e2 => tm_app (lift e1) (lift e2)
   | tm_abs A e => tm_abs A (lift e)
-  end.
+  end. *)
+Definition tm_subst {V} (e : tm ^V) (e' : tm V) : tm V :=
+  tm_subst_n 0 e e'.
 
-Fixpoint tm_subst {V} (e : tm ^V) (e' : tm V) : tm V :=
+(* Fixpoint tm_subst {V} (e : tm ^V) (e' : tm V) : tm V :=
   match e with
   | tm_var v' =>
       match v' with
@@ -93,8 +140,23 @@ Fixpoint tm_subst {V} (e : tm ^V) (e' : tm V) : tm V :=
       end
   | tm_app e1 e2 => tm_app (tm_subst e1 e') (tm_subst e2 e')
   | tm_abs A e => tm_abs A (tm_subst e (lift e'))
-  end.
+  end. *)
 
+Example subst_ex_1 : forall ty,
+  tm_subst (do 0 0) (tm_ω ty) = tm_Ω ty.
+Proof. reflexivity. Qed.
+
+Example subst_ex_2 : forall ty (e : term),
+  tm_subst (do \ty, 1 0) e = (do \ty, {lift e} 0).
+Proof. intros. cbn. reflexivity. Qed.
+
+Example subst_ex_3 : forall ty,
+  tm_subst (do 1 0) (lift (tm_id ty)) = do 0 {lift (tm_id ty)}.
+Proof. intros. cbn. reflexivity. Qed.
+
+Example subst_ex_4 : forall ty,
+  tm_subst_n 1 (do 1 0) (tm_id ty) = do {lift (tm_id ty)} 0.
+Proof. intros. cbn. reflexivity. Qed.
 
 (* Evaluation *)
 
@@ -144,13 +206,13 @@ Notation "Gamma , t" := (ctx_cons Gamma t) (at level 100, t custom stlc at level
 Reserved Notation "Gamma '|-' t ':' T"
   (at level 101, t custom stlc, T custom stlc at level 0).
 Inductive has_type : forall {V}, ctx V -> tm V -> ty -> Prop :=
-| T_Var : forall {V} Gamma (x : V) t,
+| var_has_type : forall {V} Gamma (x : V) t,
     Gamma x = t ->
     Gamma |- var x : t
-| T_Abs : forall {V} Gamma A B (e : tm ^V),
+| abs_has_type : forall {V} Gamma A B (e : tm ^V),
     Gamma, A |- e : B ->
     Gamma |- \A, e : (A -> B)
-| T_App : forall {V} (Gamma : ctx V) B A e1 e2,
+| app_has_type : forall {V} (Gamma : ctx V) B A e1 e2,
     Gamma |- e1 : (A -> B) ->
     Gamma |- e2 : A ->
     Gamma |- e1 e2 : B
@@ -195,7 +257,6 @@ Proof.
   apply ty_not_equi_recursive in H1. contradiction.
   Qed.
 
-
 Lemma val_no_steps : forall (e : term),
   val e ->
   ~ exists e', e --> e'.
@@ -233,14 +294,582 @@ Proof.
     + destruct H1; right; eexists; apply step_app1; eauto.
 Qed.
 
+
+(* Preservation *)
+
+Notation ctx' n V := (ctx (nopts n V)).
+
+Fixpoint ctx_rm
+  {V : Type} (n : nat) : ctx' (S n) V -> ctx' n V :=
+  match n with
+  | 0   => fun (ctx : ctx         ^V) (v :             V) => ctx (Some v)
+  | S n => fun (ctx : ctx' (2 + n) V) (v : nopts (S n) V) =>
+      match v with
+      | None => ctx None
+      | Some v => ctx_rm _ (fun v => ctx (Some v)) v
+      end
+  end.
+
+Fixpoint ctx_nth
+  {V : Type} (n : nat) : ctx' (S n) V -> ty :=
+  match n with
+  | 0   => fun (ctx : ctx         ^V) => ctx None
+  | S n => fun (ctx : ctx' (2 + n) V) => ctx_nth n (fun v => ctx (Some v))
+  end.
+
 Require Import Coq.Logic.FunctionalExtensionality.
 
-Lemma exchange : forall V (Gamma : ctx V) A B,
-  (do Gamma, A, B) = (do Gamma, B, A).
+Lemma ctx_decomposition : forall V (Gamma : ctx ^V),
+  Gamma = (ctx_rm 0 Gamma, {ctx_nth 0 Gamma}).
 Proof.
-  intros. apply functional_extensionality. intros.
-  destruct x; simpl.
-Admitted.
+  intros. apply functional_extensionality; intros. destruct x; reflexivity.
+  Qed.
+
+Example rm_0 : forall V (Gamma : ctx V) A,
+  ctx_rm 0 (Gamma, A) = Gamma.
+Proof. reflexivity. Qed.
+
+Example rm_1 : forall V (Gamma : ctx V) A B,
+  ctx_rm 1 (Gamma, A, B) = (Gamma, B).
+Proof. reflexivity. Qed.
+
+Fixpoint drop {V : Type} (n : nat) : ctx' n V -> ctx V :=
+  match n with
+  | 0 => fun (ctx : ctx V) => ctx
+  | S n => fun (ctx : ctx' (S n) V) => drop n (fun v => ctx (Some v))
+  end.
+
+Fixpoint lift_n {V : Type} (n : nat) : tm V -> tm' n V :=
+  match n with
+  | 0 => fun e => e
+  | S n => fun e => lift (lift_n n e)
+  end.
+
+Fixpoint lift_var_n {V : Type} (n : nat) : V -> nopts n V :=
+  match n with
+  | 0 => fun v => v
+  | S n => fun v => Some (lift_var_n n v)
+  end.
+
+(* http://citeseerx.ist.psu.edu/viewdoc/download?doi=10.1.1.447.5355&rep=rep1&type=pdf *)
+(* leave variables less than [k] untouched and remaining ones increase by [n] *)
+Fixpoint prelift_var {V : Type} { m : nat }
+  (n k : nat) (v : nopts k (nopts m V)) {struct k} : nopts k (nopts n (nopts m V)).
+destruct k.
+- exact (lift_var_n n v).
+- destruct v.
+  + exact (Some (prelift_var _ _ _ _ i)).
+  + exact None.
+Defined.
+
+(* Fixpoint prelift_var {V : Type} { m : nat }
+  (n k : nat) (v : nopts (k + m) V) {struct k} : nopts (n + (k + m)) V.
+destruct k; cbn in *.
+- apply (lift_var_n n) in v.
+  induction n; cbn in *.
+  + apply v.
+  + destruct v.
+    apply IHn in i. apply Some. apply i.
+    apply None.
+-  cut ((n + S (k + m)) = S (n + (k + m))); intros; try lia; rewrite H; clear H.
+  cbn; destruct v.
+  + apply prelift_var with (n := n) in i.
+    apply (Some i).
+  + apply None.
+Defined. *)
+
+Fixpoint prelift {V : Type} {m : nat}
+  (n k : nat) (t : tm' k (nopts m V)) {struct t} : tm' k (nopts n (nopts m V)) :=
+  match t with
+  | do var v => do var {prelift_var n k v}
+  | do e1 e2 => do {prelift n k e1} {prelift n k e2}
+  | do \t, e => do \t, {prelift n (S k) e}
+  end.
+
+(* Fixpoint prelift {V : Type} {m : nat}
+  (n k : nat) (t : tm' (k + m) V) {struct t} : tm' (n + (k + m)) V.
+refine (
+  match t with
+  | do var v => do var {prelift_var n k v}
+  | do e1 e2 => do {prelift _ _ n k e1} {prelift _ _ n k e2}
+  | do \t, e => do \t, _ (*{prelift n (S k) e} *)
+  end
+).
+apply (prelift _ _ n (S k)) in e.
+cut ((n + (S k + m)) = S (n + (k + m))); intros; try lia; rewrite H in *; clear H.
+exact e.
+Defined. *)
+
+(* Definition prelift' {V : Type} {m : nat}
+  (n k : nat) (t : tm' m V) : tm' (if lt_dec m k then m else n + m) V.
+destruct (lt_dec m k).
+- exact t.
+- assert (k <= m). lia.
+  assert (m = (k + (m - k))). lia. rewrite H0 in t.
+  apply (prelift n k) in t.
+  cut ((n + (k + (m - k))) = n + m); intros; try lia. rewrite H1 in t.
+  exact t.
+Defined. *)
+
+Example prelift_ex1 : forall {V : Type},
+  @prelift V 2 2 1 (do 0 1 2) = (do 0 3 4).
+Proof. reflexivity. Qed.
+
+Fixpoint prelift_ctx {V : Type} {m : nat}
+  (n k : nat) (ctx : ctx' (k + m) V) {struct t} : ctx' (n + (k + m)) V.
+
+Record Tm V := buildT
+  { _ctx: ctx V
+  ; _term: tm V
+  ; _type: ty
+  ; _typing: _ctx |- _term : _type
+  }.
+Notation Tm' n V := (Tm (nopts n V)).
+
+Definition Lift {V : Type} {m : nat} (n k : nat) (M : Tm' (k + m)) :
+  { N : Tm' (n + (k + m))
+  | _ctx N = liftedEnv n (_ctx M) k /\
+    _term N = prelift_aux n (_term M) k /\
+    _type N = _type M
+  }.
+
+Definition Lift_n {V : Type} (n : nat) (M: Tm V):
+  { N: Tm
+  | _ctx N = liftedEnv n (_ctx M) k /\
+    _term N = prelift_aux n (_term M) k /\
+    _type N = _type M
+  }.
+
+Lemma drop_S : forall V n (Gamma : ctx' n V) A,
+  drop (S n) (Gamma, A) = drop n Gamma.
+Proof. intros. cbn. reflexivity. Qed.
+
+Lemma ctx_inv : forall V (GammaA : ctx ^V),
+  exists Gamma A, GammaA = (Gamma, A).
+Proof.
+  intros.
+  exists (fun v => GammaA (Some v)).
+  exists (GammaA None).
+  apply functional_extensionality. intros [v|]; reflexivity.
+  Qed.
+
+Ltac ctxinv H G A := 
+  let e := fresh "e" in
+  let Heqe := fresh "Heqe" in
+  let Heq := fresh "Heq" in
+  remember (ctx_inv _ H) as e eqn:Heqe; clear Heqe; destruct e as [G [A Heq]]; subst.
+
+Ltac appauto IHe1 IHe2 :=
+  econstructor;
+  [ eapply IHe1; eauto
+  | eapply IHe2; eauto
+  ].
+
+(* Weakening : var *)
+
+Lemma weakening_var : forall V (e : tm V) Gamma A t v,
+  e = tm_var v ->
+  Gamma    |-       e  : t ->
+  Gamma, A |- {lift e} : t.
+Proof. intros. subst. cbn. inv H0. constructor. reflexivity. Qed.
+
+Lemma lift_var : forall V (v : V) n,
+  exists v',
+  lift_n n (tm_var v) = tm_var v'.
+Proof.
+  induction n; intros; cbn.
+  - eexists; eauto.
+  - destruct IHn. eexists. rewrite H. reflexivity.
+  Qed.
+
+Lemma weakening_var_n : forall V n (e : tm V) Gamma t v,
+  e = tm_var v ->
+  drop n Gamma |- e : t ->
+  Gamma |- {lift_n n e} : t.
+Proof.
+  induction n; intros; subst. auto.
+  subst. cbn.
+  ctxinv Gamma G A. 
+  rewrite drop_S in H0. eapply IHn in H0; eauto.
+  set (HH := lift_var); edestruct HH; clear HH. rewrite H in *.
+  eapply weakening_var; eauto.
+  Qed.
+
+
+(* Weakening *)
+
+Definition simple_cast {T1 T2 : Type} (H : T1 = T2) (x : T1) : T2 :=
+  eq_rect T1 (fun T3 : Type => T3) x T2 H.
+
+(* Fixpoint coerce :
+  JMeq *)
+
+
+Lemma weakening_n : forall V n (e : tm V) Gamma t,
+  drop n Gamma |- e : t ->
+  Gamma |- {lift_n n e} : t.
+Proof with cbn in *.
+  induction e; intros; inv H.
+  - eapply weakening_var_n; eauto.
+  - assert (lift_n n (do e1 e2) = do {lift_n n e1} {lift_n n e2}). admit.
+    rewrite H1.
+    appauto IHe1 IHe2.
+  - 
+    (* remember (lift_n n e).
+    assert ((iter Type n option (option V)) = option (iter Type n option V)). admit.
+    rewrite H0 in t0. *)
+    (* assert ((lift_n n (do \t, e)) = do \t, {lift_n n e}). *)
+  
+    induction n. cbn in *; auto.
+
+    assert (iter Type (S n) option V = option (iter Type n option V)). admit.
+    (* cbn in Gamma. *)
+    replace (iter Type (S n) option V) with (option (iter Type n option V)).
+
+    cbn in *.
+    assert (tm' n ^V = tm ^ (nopts n V)). admit.
+    assert (lift (lift_n n (do \ t, e)) ~= lift_n n (lift (do \ t, e))). admit.
+    subst H1.
+    remember (simple_cast H0 (lift_n n (lift (do \ t, e)))) as lam.
+    unfold simple_cast in Heqlam.
+    apply (simple_cast H0) in Heqlam.
+    
+    (* rewrite <- H0 in *. *)
+    remember (lift_n n (lift (do \ t, e))). dependent rewrite -> H0 in t0. subst.
+    dependent rewrite -> H1. JMeq
+  
+      induction n; cbn in *.
+    + appauto H H0.
+    + cbn.
+
+  - intros. cbn in Gamma.
+    remember (ctx_inv _ Gamma); clear Heqe0; destruct e0 as [G [A Heq]]; subst.
+    apply IHn in H...
+    rewrite drop_S in H. apply IHn in H.
+
+  induction n, e; auto; intros.
+  - inv H...
+  - intros... auto.
+  - intros... 
+  Qed.
+
+Lemma remove_lift : forall V (e : tm V) Gamma A t,
+  Gamma, A |- {lift e} : t ->
+  Gamma    |-       e  : t.
+Proof with cbn in *.
+  dependent induction e; intros; cbn in *; inv H.
+  - auto.
+  - econstructor.
+    eapply IHe1; eauto.
+    eapply IHe2; eauto.
+  - inv H.
+  
+    inv e. cbn in *.
+    + constructor.
+      destruct v...
+      * apply IHe in H. constructor. inv H... reflexivity.
+      * inv H. auto.
+    + constructor.
+      inv H. econstructor. apply IHe.
+    + constructor. inv e; 
+    apply IHe in H.
+  Qed.
+
+Lemma weakening : forall V (e : tm V) Gamma A t,
+  Gamma    |-       e  : t ->
+  Gamma, A |- {lift e} : t.
+Proof with cbn in *.
+  dependent induction e; intros; cbn in *; inv H.
+  - auto.
+  - econstructor.
+    eapply IHe1; eauto.
+    eapply IHe2; eauto.
+  - inv e...
+    + constructor. destruct v...
+      * inv H... constructor... reflexivity.
+      * inv H. auto.
+    + 
+  
+    econstructor.
+    eapply IHe in H.
+    eapply IHe.
+  Qed.
+
+Fixpoint optionn n (X : Type) : Type :=
+  match n with
+  | 0 => X
+  | S n => option (optionn n X)
+  end.
+
+Fixpoint liftn n (t : term) : tm (optionn n Void) :=
+  match n with
+  | 0 => t
+  | S n => lift (liftn n t)
+  end.
+
+(* Inductive hole : forall {V}, ctx ^V -> ctx V -> ty -> tm V -> term -> Prop :=
+| hole_0 : forall A e,
+    hole (emp  , A)  emp        A       e  e
+| hole_S : forall {V} (Gamma' : ctx V) Gamma A t e e',
+    hole  Gamma      Gamma'     A       e  e' ->
+    hole (Gamma, t) (Gamma', t) A (lift e) e'
+. *)
+
+Inductive hole : forall {V}, ctx ^V -> ctx V -> ty -> nat -> Prop :=
+| hole_0 : forall A,
+    hole (emp  , A)  emp        A    0
+| hole_S : forall {V} (Gamma' : ctx V) Gamma A t n,
+    hole  Gamma      Gamma'     A    n ->
+    hole (Gamma, t) (Gamma', t) A (S n)
+.
+
+Lemma hole_inv : forall V (GammaA : ctx ^V) Gamma A n,
+  hole GammaA Gamma A n ->
+  exists Gamma' B, GammaA = (Gamma', B).
+Proof.
+  intros. inv H; eexists; eexists; eauto.
+  Qed.
+
+(* Inductive hole : forall {V}, ctx V -> ty -> ctx V -> ty -> tm V -> term -> Prop :=
+| hole_0 : forall A e,
+    hole emp A  emp        A       e  e
+| hole_S : forall {V} (Gamma' : ctx V) Gamma A t e e',
+    hole  Gamma      Gamma'     A       e  e' ->
+    hole Gamma t (Gamma', t) A (lift e) e'
+. *)
+
+Lemma discriminate_ctx : forall V (Gamma1 : ctx V) Gamma2 A1 A2,
+  (Gamma1, A1) = (Gamma2, A2) ->
+  Gamma1 = Gamma2 /\ A1 = A2.
+Proof with (simpl in *; assumption).
+  intros.
+  split.
+  - apply functional_extensionality; intro v.
+    eapply equal_f with (x := Some v) in H...
+  - eapply equal_f with (x := None) in H...
+  Qed.
+
+(* TODO notation for substitution `e [0 := e']` *)
+
+Lemma subst_var_preservation :
+  forall n (x : nopts n ^Void) (e' : term) Gamma B,
+  Gamma |- var x : B ->
+  emp |- e' : {ctx_nth n Gamma} ->
+  ctx_rm n Gamma |- { tm_subst_n n (tm_var x) e' } : B.
+Proof.
+  induction n; intros; cbn in *; inv H; destruct x; cbn in *; auto.
+  - admit.
+  - eapply IHn in H0 as H1; eauto.
+  Qed.
+
+Lemma subst_preservation_clean :
+  forall V n (e : tm' n V) (e' : term) E Gamma B,
+  V = (^Void)%type ->
+  E ~= e ->
+  Gamma |- E : B ->
+  emp |- e' : {ctx_nth n Gamma} ->
+  ctx_rm n Gamma |- { tm_subst_n n E e' } : B.
+Proof with simpl in *.
+  dependent induction n; dependent induction e; intros; subst...
+  - inv H1. destruct v; auto.
+    admit.
+  - inv H1.
+    econstructor.
+    eapply IHe1; eauto.
+    eapply IHe2; eauto.
+  - inv H1.
+    econstructor.
+    eapply IHe.
+Qed.
+
+Lemma subst_preservation_clean :
+  forall n (e : tm' n ^Void) (e' : term) Gamma B,
+  Gamma |- e : B ->
+  emp |- e' : {ctx_nth n Gamma} ->
+  ctx_rm n Gamma |- { tm_subst_n n e e' } : B.
+Proof with simpl in *.
+  induction n; dependent induction e; simpl; intros.
+  - destruct v. contradiction.
+    inv H...
+    admit.
+  - inv H.
+    econstructor.
+    eapply IHe1; eauto.
+    eapply IHe2; eauto.
+  - inv H.
+    econstructor. cbn in *.
+    eapply IHe in H0 as H2.
+    eapply IHe.
+Qed.
+
+Lemma subst_preservation_qux : forall W (e : tm W) V E,
+  W = (^V)%type ->
+  E ~= e ->
+  forall (Gamma1 : ctx V) t B,
+  Gamma1, t |- E : B -> forall Gamma e' lifted_e' A,
+  hole (Gamma1, t) Gamma A lifted_e' e' ->
+  emp |- e' : A ->
+  Gamma |- { tm_subst E lifted_e' } : B.
+Proof.
+  induction e.
+  - intros. subst.
+    simpl. destruct v.
+    + inv H1. simpl in *.
+      dependent induction H2. contradiction.
+      apply discriminate_ctx in x as [Heq1 Heq2]; subst.
+      apply hole_inv in H2 as H22; destruct H22 as [GammaX [C Heq]]; subst.
+      destruct v; simpl.
+      constructor. simpl. admit.
+      admit.
+    + inv H1. simpl. dependent induction H2.
+      * assert (A = t). admit. subst.
+        assumption.
+        (* inv H1. simpl. assumption. *)
+      * apply discriminate_ctx in x as [Heq1 Heq2]. subst.
+        (* inv H1. simpl in *. *)
+        assert (Gamma' |- e : t).
+        apply hole_inv in H2 as H22; destruct H22 as [GammaX [C Heq]]; subst.
+        apply IHhole with (GammaX); auto.
+        admit.
+        admit.
+  - intros; subst; simpl.
+    inv H1.
+    econstructor.
+    eapply IHe1; eauto.
+    eapply IHe2; eauto.
+  - intros; subst; simpl.
+    inv H1.
+    constructor.
+    eapply IHe; eauto.
+    constructor. auto.
+Qed.
+
+Lemma subst_preservation_aux : forall W (e : tm W) V E,
+  W = (^V)%type ->
+  E ~= e ->
+  forall (GammaA : ctx ^V) B,
+  GammaA |- E : B -> forall Gamma e' lifted_e' A,
+  hole GammaA Gamma A lifted_e' e' ->
+  emp |- e' : A ->
+  Gamma |- { tm_subst E lifted_e' } : B.
+Proof.
+  induction e.
+  - intros. subst. simpl.
+    inv H1.
+    dependent induction H2.
+    + destruct v; simpl; auto.
+    + destruct v; simpl.
+      apply IHhole with (o) in H3 as H.
+      (* apply hole_inv in H2 as H22; destruct H22 as [GammaX [C Heq]]; subst. *)
+      destruct o; simpl in *.
+      admit.
+      inv H2. simpl in *.
+
+    apply hole_inv in H2 as H22; destruct H22 as [GammaX [C Heq]]; subst.
+    destruct v; simpl in *.
+    (* apply hole_inv in H2 as H22. destruct H22 as [Gamma' [C Heq]]. subst. *)
+    (* inv H1. simpl. *)
+    (* generalize dependent H3. *)
+    (* apply hole_inv in H2 as H22. destruct H22 as [Gamma' [C Heq]]. subst. *)
+    dependent induction H2.
+    (* intros; subst; simpl. *)
+    + inv H1. simpl. 
+      (* assert (A = C). admit. *)
+      (* subst. rewrite <- x. *)
+      destruct v; auto.
+    + 
+      (* simpl in *. *)
+      destruct v; simpl; auto.
+      * inv H1.
+        simpl in *.
+        apply (IHhole o) in H3 as H4; auto.
+        destruct o.
+        constructor. simpl. admit.
+        constructor. simpl.
+        (* apply hole_inv in H2 as H22. destruct H22 as [Gamma'' [D Heq]]. subst. *)
+        (* simpl in *. apply (IHhole o Gamma'' D) in H3 as H4. destruct o; simpl in *. *)
+        simpl in *. apply (IHhole o) in H3 as H4. destruct o; simpl in *.
+        admit.
+        apply hole_inv in H2 as H22. destruct H22 as [Gamma'' [D Heq]]. subst.
+        constructor. simpl. 
+    (* inv H1. induction H2.
+    + destruct v; auto.
+    + destruct v.
+      specialize IHhole with o. apply IHhole in H3. simpl in *.
+      destruct o; simpl.
+      * constructor. inv H3. simpl. assumption.
+      * constructor. inv H3; simpl; auto.
+        inv H2. contradiction.
+    destruct v. admit. *)
+  - intros; subst; simpl.
+    inv H1.
+    econstructor.
+    eapply IHe1; eauto.
+    eapply IHe2; eauto.
+  - intros; subst; simpl.
+    inv H1.
+    constructor.
+    eapply IHe; eauto.
+    constructor. auto.
+
+  intros W e. GammaA e B He.
+  dependent induction He; intros.
+  - admit.
+  - simpl. constructor.
+Qed.
+
+Lemma subst_preservation : forall V (Gamma : ctx V) GammaA lifted_e' e' A,
+  hole GammaA Gamma A lifted_e' e' ->
+  emp |- e' : A -> forall e B,
+  GammaA |- e : B ->
+  forall W (GammaE : ctx W) E,
+  W = (^V)%type ->
+  GammaE ~= GammaA ->
+  E ~= e ->
+  Gamma |- { tm_subst E lifted_e' } : B.
+Proof.
+  intros V Gamma GammaA lifted_e' e' A Hhole.
+  induction Hhole.
+  - intros He. dependent induction e0; intros; simpl; subst.
+    + inv H. destruct v. contradiction. simpl. assumption.
+    + inv H. simpl.
+      econstructor.
+      eapply IHe0_1; eauto.
+      eapply IHe0_2; eauto.
+    + inv H. 
+      simpl. constructor.
+      eapply IHe0.
+
+  
+  intros B Hhole He He'.
+  induction Hhole.
+
+  intros V Gamma GammaA e lifted_e' e' A B Hhole He He'.
+  dependent induction He.
+  - admit.
+  - simpl. constructor.
+Qed.
+
+Lemma subst_preservation_0 : forall W (e : tm W), forall V A B (Gamma : ctx V) E,
+  W = (^V)%type ->
+  E ~= e ->
+  Gamma, A |- E : B -> forall e',
+  Gamma |- e' : A ->
+  Gamma |- { tm_subst E e' } : B.
+Proof.
+  induction e; intros; subst.
+  - admit.
+  - admit.
+  - simpl. inv H1.
+    constructor.
+    assert (Gamma, t |- {lift e'} : A). admit.
+    eapply IHe; auto.
+  intros V Gamma e.
+  dependent induction e; intros A B He e' He'; inv He.
+  - admit.
+  - admit.
+  - simpl.
+Abort.
 
 Lemma subst_preservation_1 : forall V (Gamma : ctx V) e A B,
   Gamma, A |- e : B -> forall e',
